fix to msg_eq that we discussed but I still think it's worth a PR (#98)
* fix to msg_eq that we discussed but I still think it's worth a PR

* Update coqproject to include example file.  got dropped somehow

* Fix problems from reworked message equality.

KeyManagement/MessageEq.v
@@ -27,12 +27,18 @@ Import IdealWorld.IdealNotations.
 (* assumes that there is a shadow copy of the built message in every store in the cipherheap *)
 (* potential major refactor for usage/id/sym interraction?*)
 
-Fixpoint content_eq  {t__rw t__iw} (m__rw : RealWorld.message.message t__rw) (m__iw : IdealWorld.message.message t__iw) : Prop :=
+Fixpoint content_eq  {t__rw t__iw} (m__rw : RealWorld.message.message t__rw) (m__iw : IdealWorld.message.message t__iw) gks : Prop :=
   match (m__rw, m__iw) with
   | (RealWorld.message.Content c__rw, IdealWorld.message.Content c__iw) => c__rw = c__iw
-  | (RealWorld.message.Permission _, IdealWorld.message.Permission _) => True
+  | (RealWorld.message.Permission (id, _) , IdealWorld.message.Permission (IdealWorld.construct_access a _)) =>
+    match (gks $? id) with
+    | Some (Keys.MkCryptoKey id _ Keys.SymKey) => a = (IdealWorld.construct_permission true true)
+    | Some (Keys.MkCryptoKey id Keys.Signing Keys.AsymKey) => a = (IdealWorld.construct_permission true false)
+    | Some (Keys.MkCryptoKey id Keys.Encryption Keys.AsymKey) => a = (IdealWorld.construct_permission false true)
+    | _ => False
+    end
   | (RealWorld.message.MsgPair m__rw1 m__rw2, IdealWorld.message.MsgPair m__iw1 m__iw2) =>
-    content_eq m__rw1 m__iw1 /\ content_eq m__rw2 m__iw2
+    content_eq m__rw1 m__iw1 gks /\ content_eq m__rw2 m__iw2 gks
   | _ => False
   end.
 
@@ -50,14 +56,14 @@ Inductive  message_eq : forall {A B t},
   RealWorld.crypto t -> RealWorld.universe A B ->
   IdealWorld.message.message t -> IdealWorld.universe A -> IdealWorld.channel_id -> Prop :=
 | ContentCase : forall {A B t}  (U__rw : RealWorld.universe A B) U__iw (m__rw : RealWorld.message.message t) m__iw ch_id user_data,
-    content_eq m__rw m__iw
+    content_eq m__rw m__iw U__rw.(RealWorld.all_keys)
     -> (forall u, U__iw.(IdealWorld.users) $? u  = Some user_data
             -> resolve_perm user_data.(IdealWorld.perms) ch_id = Some (IdealWorld.construct_permission true true))
     -> message_eq (RealWorld.Content m__rw) U__rw m__iw U__iw ch_id
 | CryptoSigCase : forall {A B t} (U__rw : RealWorld.universe A B) U__iw (m__iw : IdealWorld.message.message t) c_id ch_id k__sign
                     (m__rw : RealWorld.message.message t) b__iw honestk u_id msg_seq,
     U__rw.(RealWorld.all_ciphers) $? c_id = Some (RealWorld.SigCipher k__sign u_id msg_seq m__rw)
-    -> content_eq m__rw m__iw
+    -> content_eq m__rw m__iw U__rw.(RealWorld.all_keys)
     -> honestk = RealWorld.findUserKeys (U__rw.(RealWorld.users))
     -> (forall u data__rw data__iw,
 	                     U__rw.(RealWorld.users) $? u = Some data__rw
@@ -65,12 +71,12 @@ Inductive  message_eq : forall {A B t},
                           ->  RealWorld.honest_key honestk k__sign
           (*sign key is honest.  honest key : find user keys on all users*)
             -> (data__rw.(RealWorld.key_heap) $? k__sign = Some true
-               <-> resolve_perm data__iw.(IdealWorld.perms) ch_id = Some (IdealWorld.construct_permission true b__iw)))
+               -> resolve_perm data__iw.(IdealWorld.perms) ch_id = Some (IdealWorld.construct_permission true b__iw)))
     -> message_eq (RealWorld.SignedCiphertext c_id) U__rw m__iw U__iw ch_id
 | CryptoSigEncCase : forall {A B t} (U__rw : RealWorld.universe A B) U__iw (m__iw : IdealWorld.message.message t) c_id ch_id k__sign k__enc
                        (m__rw : RealWorld.message.message t) honestk u_id msg_seq,
     U__rw.(RealWorld.all_ciphers) $? c_id = Some (RealWorld.SigEncCipher k__sign k__enc u_id msg_seq m__rw)
-    -> content_eq m__rw m__iw
+    -> content_eq m__rw m__iw U__rw.(RealWorld.all_keys)
     -> honestk = RealWorld.findUserKeys (U__rw.(RealWorld.users))
     -> (forall u data__rw data__iw b__rwenc,
 	                     U__rw.(RealWorld.users) $? u = Some data__rw
@@ -79,5 +85,5 @@ Inductive  message_eq : forall {A B t},
                           -> RealWorld.honest_key honestk k__enc
             -> ((data__rw.(RealWorld.key_heap) $? k__sign = Some true
                 /\ data__rw.(RealWorld.key_heap) $? k__enc = Some b__rwenc)
-               <-> resolve_perm data__iw.(IdealWorld.perms) ch_id = Some (IdealWorld.construct_permission b__rwenc true)))
+               -> resolve_perm data__iw.(IdealWorld.perms) ch_id = Some (IdealWorld.construct_permission b__rwenc true)))
     -> message_eq (RealWorld.SignedCiphertext c_id) U__rw m__iw U__iw ch_id.
